Location in parser done (up to a cheat)

examples/formal-languages/context-free/grammarScript.sml
@@ -2,7 +2,7 @@ open HolKernel Parse boolLib bossLib
 
 open boolSimps lcsymtacs
 
-open listTheory pred_setTheory finite_mapTheory
+open listTheory pred_setTheory finite_mapTheory locationTheory
 
 val FLAT_APPEND = rich_listTheory.FLAT_APPEND
 val rveq = rpt BasicProvers.VAR_EQ_TAC
@@ -19,7 +19,7 @@ val isTOK_def = Define`(isTOK (TOK tok) = T) ∧ (isTOK (NT n) = F)`
 val _ = export_rewrites ["isTOK_def"]
 
 val destTOK_def = Define`
-  (destTOK (TOK tk) = SOME tk) ∧
+  (destTOK (TOK tk, _) = SOME tk) ∧
   (destTOK _ = NONE)
 `;
 val _ = export_rewrites ["destTOK_def"]
@@ -31,17 +31,19 @@ val _ = Datatype`
 |> `;
 
 val _ = Datatype`
-  parsetree = Lf (('a,'b) symbol)
-            | Nd ('b inf) (parsetree list)
+  parsetree = Lf (('a,'b) symbol # locs)
+            | Nd ('b inf # locs) (parsetree list)
 `;
 
 val ptree_size_def = tDefine "ptree_size" `
-  (ptree_size (Lf tok) = 1) ∧
+  (ptree_size (Lf (tok, l)) = 1) ∧
   (ptree_size (Nd nt children) = 1 + SUM (MAP ptree_size children))
-` (WF_REL_TAC `measure (parsetree_size (K 1) (K 1))` THEN
-   Induct_on `children` THEN
-   SRW_TAC [][definition "parsetree_size_def"] THEN1 DECIDE_TAC THEN
-   RES_TAC THEN POP_ASSUM (Q.SPEC_THEN `nt` MP_TAC) THEN
+`
+(WF_REL_TAC `measure (parsetree_size (K 1) (K 1))` THEN
+   Induct_on `children` 
+   THEN SRW_TAC [][definition "parsetree_size_def"] 
+   THEN1 DECIDE_TAC THEN
+   RES_TAC THEN POP_ASSUM (Q.SPECL_THEN [`p_2`, `p_1'`, `p_1`] MP_TAC) THEN
    DECIDE_TAC)
 
 val ptree_size_def = save_thm(
@@ -50,8 +52,8 @@ val ptree_size_def = save_thm(
 val _ = export_rewrites ["ptree_size_def"]
 
 val ptree_head_def = Define`
-  (ptree_head (Lf tok) = tok) ∧
-  (ptree_head (Nd nt children) = NT nt)
+  (ptree_head (Lf (tok,l)) = tok) ∧
+  (ptree_head (Nd (nt,l) children) = NT nt)
 `;
 val _ = export_rewrites ["ptree_head_def"]
 
@@ -59,7 +61,7 @@ val noneval = Lib.with_flag (computeLib.auto_import_definitions,false)
 fun tzDefine nm q tac = noneval (tDefine nm q) tac
 val valid_ptree_def = tzDefine "valid_ptree" `
   (valid_ptree G (Lf _) ⇔ T) ∧
-  (valid_ptree G (Nd nt children) ⇔
+  (valid_ptree G (Nd (nt,l) children) ⇔
     nt ∈ FDOM G.rules ∧ MAP ptree_head children ∈ G.rules ' nt ∧
     ∀pt. pt ∈ set children ⇒ valid_ptree G pt)`
   (WF_REL_TAC `measure (ptree_size o SND)` THEN
@@ -68,7 +70,7 @@ val valid_ptree_def = tzDefine "valid_ptree" `
 val _ = export_rewrites ["valid_ptree_def"]
 
 val ptree_fringe_def = tDefine "ptree_fringe" `
-  (ptree_fringe (Lf t) = [t]) ∧
+  (ptree_fringe (Lf (t,_)) = [t]) ∧
   (ptree_fringe (Nd _ children) = FLAT (MAP ptree_fringe children))
 ` (WF_REL_TAC `measure ptree_size` THEN Induct_on `children` THEN
    SRW_TAC [][ptree_size_def] THEN1 DECIDE_TAC THEN
@@ -155,7 +157,7 @@ val ptree_ind = save_thm(
 val valid_ptree_derive = store_thm(
   "valid_ptree_derive",
   ``∀pt. valid_ptree G pt ⇒ derives G [ptree_head pt] (ptree_fringe pt)``,
-  ho_match_mp_tac ptree_ind >> rw[] >> fs[] >>
+  ho_match_mp_tac ptree_ind >> rw[] >> Cases_on`pt` >> fs[] >>
   match_mp_tac RTC1 >> qexists_tac `MAP ptree_head l` >> rw[] >>
   qpat_x_assum `SS ∈ G.rules ' s` (K ALL_TAC) >> Induct_on `l` >> rw[] >>
   fs[DISJ_IMP_THM, FORALL_AND_THM] >>
@@ -204,19 +206,21 @@ val fringe_element = store_thm(
   "fringe_element",
   ``∀pt p x s.
       ptree_fringe pt = p ++ [x] ++ s ⇒
-      (pt = Lf x ∧ p = [] ∧ s = []) ∨
-      ∃nt ip is ts1 xpt ts2.
-        pt = Nd nt (ts1 ++ [xpt] ++ ts2) ∧
+      ∃l. (pt = Lf (x,l) ∧ p = [] ∧ s = []) ∨
+      ∃nt l ip is ts1 xpt ts2.
+        pt = Nd (nt,l) (ts1 ++ [xpt] ++ ts2) ∧
         p = FLAT (MAP ptree_fringe ts1) ++ ip ∧
         s = is ++ FLAT (MAP ptree_fringe ts2) ∧
         ptree_fringe xpt = ip ++ [x] ++ is``,
   gen_tac >>
-  `(∃tok. pt = Lf tok) ∨ (∃sym ptl. pt = Nd sym ptl)`
-    by (Cases_on `pt` >> simp[]) >- simp[APPEND_EQ_CONS] >>
+  `(∃tok l . pt = Lf (tok,l)) ∨ (∃sym ptl. pt = Nd sym ptl)`
+    by (Cases_on `pt` >> Cases_on `p` >> simp[] ) 
+  >- simp[APPEND_EQ_CONS] >>
   simp[] >> pop_assum (K ALL_TAC) >> rpt gen_tac >>
   simp[Once FLAT_EQ_APPEND] >>
   disch_then
     (DISJ_CASES_THEN2 (qxchl [`fsp`, `fss`] strip_assume_tac) mp_tac) >| [
+    Cases_on `sym` >> simp[] >>
     qpat_x_assum `p ++ [x] = FLAT fsp` mp_tac >>
     simp[Once FLAT_EQ_APPEND] >>
     disch_then
@@ -276,9 +280,9 @@ val fringe_element = store_thm(
                      f2 = MAP ptree_fringe pt2 ∧
                      fp ++ [x] ++ fs = ptree_fringe ptx`
       by metis_tac [th,APPEND_ASSOC]) >>
+    Cases_on `sym` >> simp[] >>  
     map_every qexists_tac [`fp`, `fs`, `pt1`, `ptx`, `pt2`] >>
-    simp[] >> rw[] >> fs[]
-  ]);
+    simp[] >> rw[] >> fs[] ]);
 
 val derive_fringe = store_thm(
   "derive_fringe",
@@ -287,18 +291,23 @@ val derive_fringe = store_thm(
       ∃pt'.
          ptree_head pt' = ptree_head pt ∧ valid_ptree G pt' ∧
          ptree_fringe pt' = sf``,
-  ho_match_mp_tac ptree_ind >> rw[]
-  >- (fs[derive_def, APPEND_EQ_CONS] >>
-      qexists_tac `Nd sym (MAP Lf sf)` >> rw[MEM_MAP]
+  ho_match_mp_tac ptree_ind>> rw[]
+  >- (
+      Cases_on `pt` >>
+      fs[derive_def, APPEND_EQ_CONS] >>
+      qexists_tac `Nd (sym,unknown_loc) (MAP (\x. Lf(x, unknown_loc)) sf)`
+      >> rw[MEM_MAP,ptree_fringe_def]
       >- rw[MAP_MAP_o, combinTheory.o_DEF]
       >- rw[] >>
       rw[MAP_MAP_o, combinTheory.o_DEF] >>
       pop_assum (K ALL_TAC) >> Induct_on `sf` >> rw[]) >>
+  Cases_on `pt` >>
   qpat_x_assum `derive G XX YY` mp_tac >>
   simp[derive_def] >>
   disch_then (qxchl [`pfx`, `nt`, `rhs`, `sfx`] strip_assume_tac) >>
   qspecl_then [`Nd s l`, `pfx`, `NT nt`, `sfx`] mp_tac fringe_element >>
-  simp[] >>
+  Cases_on `s` >>
+  fs[] >>
   disch_then (qxchl [`ip`, `is`, `ts1`, `xpt`, `ts2`] strip_assume_tac) >>
   rw[] >>
   fs[FLAT_APPEND, DISJ_IMP_THM, FORALL_AND_THM] >>
@@ -308,7 +317,7 @@ val derive_fringe = store_thm(
     (fn th => first_x_assum
                 (fn impth => mp_tac (MATCH_MP impth th))) >>
   disch_then (qxch `pt'` strip_assume_tac) >>
-  qexists_tac `Nd s (ts1 ++ [pt'] ++ ts2)` >>
+  qexists_tac `Nd (q,r') (ts1 ++ [pt'] ++ ts2)` >>
   simp[FLAT_APPEND, DISJ_IMP_THM, FORALL_AND_THM]);
 
 val ptrees_derive_extensible = store_thm(
@@ -334,7 +343,7 @@ val singleton_derives_ptree = store_thm(
   "singleton_derives_ptree",
   ``derives G [h] sf ⇒
     ∃pt. valid_ptree G pt ∧ ptree_head pt = h ∧ ptree_fringe pt = sf``,
-  strip_tac >> qspec_then `Lf h` mp_tac ptrees_derive_extensible >> simp[]);
+  strip_tac >> qspec_then `Lf (h,l)` mp_tac ptrees_derive_extensible >> simp[]);
 
 val derives_language = store_thm(
   "derives_language",
@@ -342,7 +351,7 @@ val derives_language = store_thm(
   rw[language_def, EXTENSION, complete_ptree_def] >> eq_tac
   >- metis_tac[valid_ptree_derive] >>
   strip_tac >>
-  qspecl_then [`Lf (NT G.start)`, `MAP TOK x`] mp_tac
+  qspecl_then [`Lf (NT G.start, unknown_loc)`, `MAP TOK x`] mp_tac
     ptrees_derive_extensible >> simp[] >>
   disch_then (qxch `pt` strip_assume_tac) >> qexists_tac `pt` >>
   simp[] >> asm_simp_tac (srw_ss() ++ DNF_ss) [MEM_MAP]);
